

Calcolare $145^{145} \bmod 13$

$$145^{145 \bmod \phi(13)} \equiv 145^{145 \bmod 12} \equiv 145 \bmod 13 \equiv 2$$

Verificare che $11^{13} \bmod 17 = 17^{13} \bmod 11$

$$\begin{aligned} 11^{13} \bmod 17 &= [(11 \bmod 17) \cdot ((11^2)^6 \bmod 17)] \bmod 17 = \\ &= \{11 \cdot [(121 \bmod 17)^6 \bmod 17]\} \bmod 17 = \\ &= \{11 \cdot [2^6 \bmod 17]\} \bmod 17 = \{11 \cdot 13\} \bmod 17 = 7 \end{aligned}$$

$$\begin{aligned} 17^{13} \bmod 11 &= 17^{13 \bmod \phi(11)} \bmod 11 = 17^3 \bmod 11 = (17 \bmod 11)^3 \bmod 11 = \\ &= 6^3 \bmod 11 = [6 \bmod 11] \cdot [6^2 \bmod 11] \bmod 11 = (6 \cdot 3) \bmod 11 = 7 \end{aligned}$$

INVERSO MOD. DI $11 \bmod 7$

$$(n \bmod m)^{\phi(m)-1} \bmod m$$

$$(11 \bmod 7)^5 \bmod 7 = 4^5 \bmod 7 = [(4^2 \bmod 7) \cdot (4^2 \bmod 7) \cdot (4 \bmod 7)] \bmod 7 = 2$$

INVERSO MOD. DI $30 \bmod 11$

$$\begin{aligned} (30 \bmod 11)^{\phi(11)-1} \bmod 11 &= 8^9 \bmod 11 = [(8 \bmod 11) \cdot (64^4 \bmod 11)] \bmod 11 \\ &= [8 \cdot (64 \bmod 11)^4 \bmod 11] \bmod 11 = \\ &= [8 \cdot (9^4 \bmod 11)] \bmod 11 = [8 \cdot (9^2 \bmod 11)^2 \bmod 11] \bmod 11 \\ &= 7 \end{aligned}$$

VERIFICO:

$$(7 \cdot 30) \bmod 11 = 1 \bmod 11$$

$$1 = 1$$

$$9^{100} \bmod 8 = 9^{100 \bmod \phi(8)} \bmod 8 = 9^{100 \bmod 4} \bmod 8 = 9^0 \bmod 8 = 1 \bmod 8 = 1$$

$$15^{80} \bmod 16 = 15^{80 \bmod \phi(16)} \bmod 16 = 15^{80 \bmod 8} \bmod 16 = 1$$

$$\begin{aligned} 13^{40} \bmod 19 &= 13^{40 \bmod \phi(19)} \bmod 19 = 13^{40 \bmod 18} \bmod 19 = 13^4 \bmod 19 = \\ &= [(13^2 \bmod 19) \cdot (13^2 \bmod 19)] \bmod 19 = 17^2 \bmod 19 = \\ &= (-2)^2 \bmod 19 = 4 \bmod 19 = 4 \end{aligned}$$

$$\begin{aligned} 11^{57} \bmod 23 &= 11^{57 \bmod \phi(23)} \bmod 23 = 11^{57 \bmod 22} \bmod 23 = 11^{13} \bmod 23 = \\ &= [(11 \bmod 23) \cdot (121^6 \bmod 23)] \bmod 23 = \\ &= \{ 11 \cdot [(121 \bmod 23)^6 \bmod 23] \} \bmod 23 = \\ &= \{ 11 \cdot [6^6 \bmod 23] \} \bmod 23 = \\ &= \{ 11 \cdot [(36 \bmod 23)^3 \bmod 23] \} \bmod 23 = \\ &= \{ 11 \cdot [13^3 \bmod 23] \} \bmod 23 = \\ &= \{ 11 \cdot [(169 \bmod 23) \cdot 13] \bmod 23 \} \bmod 23 = \\ &= \{ 11 \cdot [104 \bmod 23] \} \bmod 23 = (11 \cdot 12) \bmod 23 = 132 \bmod 23 = 17 \end{aligned}$$

$$7^{50} \bmod 11 = 7^{50 \bmod \phi(11)} \bmod 11 = 7^0 \bmod 11 = 1$$

$$\begin{aligned} 40^{60} \cdot 60^{40} \bmod 31 &= [(40^{60} \bmod 31) \cdot (60^{40} \bmod 31)] \bmod 31 = (60^{40} \bmod 31) \bmod 31 \\ &\cdot 40^{60} \bmod 31 = 40^{60 \bmod \phi(31)} \bmod 31 = 1 \quad \text{---} \\ &\cdot 60^{40} \bmod 31 = 60^{40 \bmod \phi(31)} \bmod 31 = 60^{10} \bmod 31 = \\ &= (60 \bmod 31)^{10} \bmod 31 = 29^{10} \bmod 31 = [(29^2 \bmod 31)^5 \bmod 31] = \\ &= (841 \bmod 31)^5 \bmod 31 = 4^5 \bmod 31 = [(4 \bmod 31) \cdot (4^4 \bmod 31)] \bmod 31 \\ &= \{ 4 \cdot [(4^3 \bmod 31) \cdot (4 \bmod 31)] \bmod 31 \} \bmod 31 = \{ 4 \cdot 8 \} \bmod 31 = 1 \\ &= 1 \bmod 31 = 1 \end{aligned}$$

$$29^{101} \bmod 31$$

$$\begin{aligned}
 &= 29^{101 \bmod \phi(31)} \bmod 31 = 29^{101 \bmod 30} \bmod 31 = 29^{11} \bmod 31 = \\
 &= [(29 \bmod 31) \cdot (29^{10} \bmod 31)] \bmod 31 = [29 \cdot (29^{10} \bmod 31)] \bmod 31 \\
 &= \{29 \cdot [(29^2 \bmod 31)^5 \bmod 31]\} \bmod 31 = \{29 \cdot [4^5 \bmod 31]\} \bmod 31 = \\
 &= \{29 \cdot [(4^3 \bmod 31)(4^2 \bmod 31)] \bmod 31\} \bmod 31 = \{29 \cdot 1\} \bmod 31 = 29
 \end{aligned}$$

$$\text{Inverso di } 49 \text{ modulo } 23$$

$$(n \bmod m)^{\phi(m)-1} \bmod m$$

$$\begin{aligned}
 (49 \bmod 23)^{\phi(23)-1} \bmod 23 &= 3^{21} \bmod 23 = (3^3 \bmod 23)^7 \bmod 23 = \\
 &= 4^7 \bmod 23 = [(4^3 \bmod 23)(4^4 \bmod 23)] \bmod 23 = \\
 &= \{18 \cdot [(4^3 \bmod 23)(4 \bmod 23)] \bmod 23\} \bmod 23 = \\
 &= \{18 \cdot [18 \cdot 4] \bmod 23\} \bmod 23 = \{18 \cdot 3\} \bmod 23 = \\
 &= 8
 \end{aligned}$$

$$\text{Inverso di } 51 \text{ modulo } 16$$

$$\begin{aligned}
 (51 \bmod 16)^{\phi(16)-1} \bmod 16 &= 3^7 \bmod 16 = [(3^3 \bmod 16)(3^3 \bmod 16)(3 \bmod 16)] \bmod 16 = \\
 &= (11 \cdot 11 \cdot 3) \bmod 16 = (11^2 \cdot 3) \bmod 16 = \\
 &= [(11^2 \bmod 16)(3 \bmod 16)] \bmod 16 = 27 \bmod 16 = 11
 \end{aligned}$$

$$\text{Inverso di } 63 \text{ modulo } 10$$

$$(63 \bmod 10)^{\phi(10)-1} \bmod 10 = 3^3 \bmod 10 = 27 \bmod 10 = 7$$

$$\text{Inverso di } 72 \text{ modulo } 5$$

$$(72 \bmod 5)^{\phi(5)-1} \bmod 5 = 2^3 \bmod 5 = 3$$

Inverso di 83 modulo 10

$$(83 \bmod 10)^{\phi(10)-1} \bmod 10 = 3^3 \bmod 10 = 7$$

Inverso di 97 modulo 11

$$\begin{aligned} (97 \bmod 11)^{\phi(11)-1} \bmod 11 &= 9^3 \bmod 11 = [(9^2 \bmod 11)(9 \bmod 11)] \bmod 11 = \\ &= \{4 \cdot [(9^2 \bmod 11)(9^2 \bmod 11) \cdot (9^2 \bmod 11)(9 \bmod 11)] \bmod 11\} \bmod 11 = \\ &= \{4 \cdot (4 \cdot 4 \cdot 4 \cdot 9) \bmod 11\} \bmod 11 = \\ &= \{4 \cdot (4^3 \cdot 9) \bmod 11\} \bmod 11 = \\ &= \{4 \cdot [(4^3 \bmod 11)(9 \bmod 11)] \bmod 11\} \bmod 11 = \\ &= \{4 \cdot (81 \bmod 11)\} \bmod 11 = (4 \cdot 4) \bmod 11 = 5 \end{aligned}$$

Inverso di 100 modulo 23

$$\begin{aligned} (100 \bmod 23)^{\phi(23)-1} \bmod 23 &= 8^{21} \bmod 23 = (8^3 \bmod 23)^7 \bmod 23 = 6^7 \bmod 23 = \\ &= [(486 \bmod 23)] \bmod 23 = 3 \bmod 23 = 3 \end{aligned}$$

$\nearrow 6^3 \cdot 6^3 \cdot 6$